feat(*) cleanup

HOTG/Arithmetics/Functions_Restrict.thy
@@ -1,6 +1,6 @@
 \<^marker>\<open>creator "Kevin Kappelmann"\<close>
 theory Functions_Restrict
-  imports HOL.HOL
+  imports Basic
 begin
 
 consts fun_restrict :: "('a \<Rightarrow> 'b) \<Rightarrow> 'c \<Rightarrow> 'a \<Rightarrow> 'b"
@@ -30,5 +30,16 @@ lemma fun_restrict_eq_if_not [simp]:
   assumes "\<not>(P x)"
   shows "f\<restriction>\<^bsub>P\<^esub> x = undefined"
   using assms unfolding fun_restrict_pred_def by auto
+
+
+overloading
+  fun_restrict_set \<equiv> "fun_restrict :: (set \<Rightarrow> 'a) \<Rightarrow> set \<Rightarrow> set \<Rightarrow> 'a"
+begin
+  definition "fun_restrict_set f X \<equiv> f\<restriction>\<^bsub>mem_of X\<^esub> :: set \<Rightarrow> 'a"
+end
+
+lemma fun_restrict_set_eq_fun_restrict [simp]: "(f :: set \<Rightarrow> 'a)\<restriction>\<^bsub>X\<^esub> = f\<restriction>\<^bsub>mem_of X\<^esub>"
+  unfolding fun_restrict_set_def by auto
+
 
 end
