HOTG/Arithmetics/Mem_Transitive_Closure.thy
@@ -1,54 +1,11 @@
+\<^marker>\<open>creator "Linghan Fang"\<close>
+\<^marker>\<open>creator "Kevin Kappelmann"\<close>
+section \<open>Transitive Closure With Respect To Membership\<close>
 theory Mem_Transitive_Closure
   imports
-    Transport.Functions_Injective
-    Functions_Restrict
     Foundation
-    Union_Intersection
+    Transfinite_Recursion
 begin
-
-(*TODO Kevin: rename to binary_relation_restrict*)
-unbundle no_restrict_syntax
-unbundle no_HOL_ascii_syntax
-
-overloading
-  fun_restrict_set \<equiv> "fun_restrict :: (set \<Rightarrow> 'a) \<Rightarrow> set \<Rightarrow> set \<Rightarrow> 'a"
-begin
-  definition "fun_restrict_set f X \<equiv> f\<restriction>\<^bsub>mem_of X\<^esub> :: set \<Rightarrow> 'a"
-end
-
-lemma fun_restrict_set_eq_fun_restrict [simp]: "(f :: set \<Rightarrow> 'a)\<restriction>\<^bsub>X\<^esub> = f\<restriction>\<^bsub>mem_of X\<^esub>"
-  unfolding fun_restrict_set_def by auto
-
-axiomatization transrec :: "((set \<Rightarrow> 'a) \<Rightarrow> set \<Rightarrow> 'a) \<Rightarrow> set \<Rightarrow> 'a"
-  where transrec_eq: "transrec f X = f ((transrec f)\<restriction>\<^bsub>X\<^esub>) X"
-
-paragraph \<open>Transitive Closure\<close>
-
-definition "image f A \<equiv> {f x | x \<in> A}"
-
-lemma image_eq_repl [simp]: "image f A = repl A f"
-  unfolding image_def by simp
-
-lemma repl_fun_restrict_eq_repl [simp]: "{f\<restriction>\<^bsub>A\<^esub> x | x \<in> A} = {f x | x \<in> A}"
-  by simp
-
-lemma injective_image_if_injective:
-  assumes "injective f"
-  shows "injective (image f)"
-  by (intro injectiveI eqI) (use assms in \<open>auto dest: injectiveD\<close>)
-
-lemma injective_if_injective_image:
-  assumes "injective (image f)"
-  shows "injective f"
-proof (rule injectiveI)
-  fix X Y assume "f X = f Y"
-  then have "image f {X} = image f {Y}" by simp
-  with assms show "X = Y" by (blast dest: injectiveD)
-qed
-
-corollary injective_image_iff_injective [iff]: "injective (image f) \<longleftrightarrow> injective f"
-  using injective_image_if_injective injective_if_injective_image by blast
-
 
 definition "mem_trans_closure \<equiv> transrec (\<lambda>f X. X \<union> (\<Union>x \<in> X. f x))"
 
@@ -72,11 +29,15 @@ lemma mem_mem_trans_closureE [elim]:
   obtains (mem) "X \<in> Y" | (mem_trans_closure) y where "y \<in> Y" "X \<in> mem_trans_closure y"
   using assms by (subst (asm) mem_trans_closure_eq_bin_union_idx_union) auto
 
-lemma mem_eq_mem_trans_closure:"X \<in> mem_trans_closure Y \<longleftrightarrow>  X \<in> Y \<or> (X\<in> (\<Union>y \<in> Y. mem_trans_closure y))"
+lemma mem_mem_trans_closure_iff_mem_or_mem:
+  "X \<in> mem_trans_closure Y \<longleftrightarrow>  X \<in> Y \<or> (X \<in> (\<Union>y \<in> Y. mem_trans_closure y))"
   by (subst mem_trans_closure_eq_bin_union_idx_union) auto
 
 lemma mem_trans_closure_empty_eq_empty [simp]: "mem_trans_closure {} = {}"
   by (simp add: mem_trans_closure_eq_bin_union_idx_union[where ?X="{}"])
+
+lemma mem_trans_closure_eq_empty_iff_eq_empty [iff]: "mem_trans_closure X = {} \<longleftrightarrow> X = {}"
+  using subset_mem_trans_closure_self by auto
 
 lemma mem_trans_closed_mem_trans_closure: "mem_trans_closed (mem_trans_closure X)"
 proof (induction X)
@@ -87,8 +48,8 @@ proof (induction X)
     then show "y \<in> mem_trans_closure X"
     proof (cases rule: mem_mem_trans_closureE)
       case mem
-      moreover have "y \<in> mem_trans_closure x" using \<open>y \<in> x\<close> subset_mem_trans_closure_self by blast
-      ultimately show ?thesis by (subst mem_trans_closure_eq_bin_union_idx_union) blast
+      have "y \<in> mem_trans_closure x" using \<open>y \<in> x\<close> subset_mem_trans_closure_self by blast
+      with mem show ?thesis by (subst mem_trans_closure_eq_bin_union_idx_union) blast
     next
       case mem_trans_closure
       with \<open>y \<in> x\<close> mem.IH show ?thesis by (subst mem_trans_closure_eq_bin_union_idx_union) blast
@@ -106,26 +67,33 @@ proof
   qed auto
 qed
 
-lemma less_asym_TC: "\<lbrakk>x < y; y < x\<rbrakk> \<Longrightarrow> False"
-  sorry
+lemma mem_trans_closure_le_if_le_if_mem_trans_closed:
+  "\<lbrakk>mem_trans_closed X;  Y \<le> X\<rbrakk> \<Longrightarrow> mem_trans_closure Y \<le> X"
+proof (induction Y)
+  case (mem Y)
+  show ?case
+  proof (cases "Y = {}")
+    case False
+    with mem have "(\<Union>y \<in> Y. mem_trans_closure y) \<le> X" by auto
+    with mem.prems show ?thesis by (simp add: mem_trans_closure_eq_bin_union_idx_union[of Y])
+  qed auto
+qed
 
-
-(*le_TC_t*)
 (*TODO Fang: prove this*)
 lemma mem_mem_trans_closure_trans:
   assumes "X \<in> mem_trans_closure Y"
   and "Y \<in> mem_trans_closure Z"
-shows "X \<in> mem_trans_closure Z"
+  shows "X \<in> mem_trans_closure Z"
 proof (rule ccontr)
   assume con:"X \<notin> mem_trans_closure Z"
-  then show False 
+  then show False
   proof -
     have "X \<notin> Z \<and> (X\<notin> (\<Union>z \<in> Z. mem_trans_closure z))"
-      using con by (auto simp: mem_eq_mem_trans_closure)
+      using con by (auto simp: mem_mem_trans_closure_iff_mem_or_mem)
     with assms(1) have "Y \<notin> Z"
       by auto
     with assms have "Y\<in> (\<Union>z \<in> Z. mem_trans_closure z)"
-      by (auto simp: mem_eq_mem_trans_closure)
+      by (auto simp: mem_mem_trans_closure_iff_mem_or_mem)
     then obtain yy where "yy \<in> Z" "Y \<in> mem_trans_closure yy" by blast
     then have "yy \<in> mem_trans_closure Z" "Y \<in> mem_trans_closure yy"
       by (auto simp: mem_mem_trans_closure_if_mem)
