HOTG/Arithmetics/Less_Than.thy
@@ -1,11 +1,35 @@
+\<^marker>\<open>creator "Linghan Fang"\<close>
+\<^marker>\<open>creator "Kevin Kappelmann"\<close>
+section \<open>Less-Than Order\<close>
 theory Less_Than
   imports
+    Transport.Binary_Relations_Antisymmetric
+    Transport.Binary_Relations_Reflexive
+    Transport.HOL_Syntax_Bundles_Groups
     Transport.HOL_Syntax_Bundles_Orders
-    Foundation
     Mem_Transitive_Closure
 begin
 
-unbundle no_HOL_ascii_syntax
+abbreviation "zero_set \<equiv> {}"
+abbreviation "one_set \<equiv> {zero_set}"
+abbreviation "two_set \<equiv> {zero_set, one_set}"
+
+bundle hotg_set_zero_syntax begin notation zero_set ("0") end
+bundle no_hotg_set_zero_syntax begin no_notation zero_set ("0") end
+
+bundle hotg_set_one_syntax begin notation one_set ("1") end
+bundle no_hotg_set_one_syntax begin no_notation one_set ("1") end
+
+bundle hotg_set_two_syntax begin notation two_set ("2") end
+bundle no_hotg_set_two_syntax begin no_notation two_set ("2") end
+
+unbundle
+  hotg_set_zero_syntax
+  hotg_set_one_syntax
+  hotg_set_two_syntax
+unbundle
+  no_HOL_ascii_syntax
+  no_HOL_groups_syntax
 
 paragraph \<open>Less-Than Order\<close>
 
@@ -19,20 +43,44 @@ unbundle no_HOL_order_syntax
 lemma lt_iff_mem_trans_closure: "X < Y \<longleftrightarrow> X \<in> mem_trans_closure Y"
   unfolding lt_def by simp
 
+lemma lt_if_mem_trans_closure:
+  assumes "X \<in> mem_trans_closure Y"
+  shows "X < Y"
+  using assms unfolding lt_iff_mem_trans_closure by simp
+
+corollary lt_if_mem:
+  assumes "X \<in> Y"
+  shows "X < Y"
+  using assms subset_mem_trans_closure_self lt_if_mem_trans_closure by auto
+
+lemma mem_trans_closure_if_lt:
+  assumes "X < Y"
+  shows "X \<in> mem_trans_closure Y"
+  using assms unfolding lt_iff_mem_trans_closure by simp
+
 lemma lt_if_lt_if_mem [trans]:
-  assumes "y \<in> Y"
-  and "Y < X"
-  shows "y < X"
+  assumes "x \<in> X"
+  and "X < Y"
+  shows "x < Y"
   using assms mem_trans_closed_mem_trans_closure unfolding lt_iff_mem_trans_closure by auto
 
 lemma lt_trans [trans]:
   assumes "X < Y"
   and "Y < Z"
-  shows "X < Y"
-  using assms mem_mem_trans_closure_trans by auto
+  shows "X < Z"
+  using assms unfolding lt_iff_mem_trans_closure by (rule mem_mem_trans_closure_trans)
 
 lemma not_lt_self [iff]: "\<not>(X < X)"
-  using lt_iff_mem_trans_closure by auto
+  unfolding lt_iff_mem_trans_closure by auto
+
+lemma not_lt_zero [iff]: "\<not>(X < 0)"
+  unfolding lt_iff_mem_trans_closure by auto
+
+lemma zero_lt_if_ne_zero [iff]:
+  assumes "X \<noteq> 0"
+  shows "0 < X"
+  using assms mem_trans_closed_mem_trans_closure
+  by (intro lt_if_mem_trans_closure empty_mem_if_mem_trans_closed) auto
 
 
 paragraph \<open>Less-Than or Equal Order\<close>
@@ -43,17 +91,101 @@ bundle hotg_le_syntax begin notation le (infix "\<le>" 60) end
 bundle no_hotg_le_syntax begin no_notation le (infix "\<le>" 60) end
 unbundle hotg_le_syntax
 
-lemma le_iff_mem_trans_closure_or_eq: "X \<le> Y \<longleftrightarrow> X \<in> mem_trans_closure Y \<or> X = Y"
-  by (simp add: le_def lt_iff_mem_trans_closure)
+lemma le_if_lt:
+  assumes "X < Y"
+  shows "X \<le> Y"
+  using assms unfolding le_def by auto
+
+lemma le_self [iff]: "X \<le> X" unfolding le_def by simp
+
+corollary reflexive_le: "reflexive (\<le>)" by auto
+
+lemma leE:
+  assumes "X \<le> Y"
+  obtains (lt) "X < Y" | (eq) "X = Y"
+  using assms unfolding le_def by auto
+
+corollary le_iff_lt_or_eq: "X \<le> Y \<longleftrightarrow> X < Y \<or> X = Y"
+  using le_if_lt leE by blast
 
 lemma le_trans [trans]:
   assumes "X \<le> Y"
   and "Y \<le> Z"
   shows "X \<le> Z"
-  using assms mem_mem_trans_closure_trans unfolding le_iff_mem_trans_closure_or_eq by auto
+  using assms lt_trans unfolding le_iff_lt_or_eq by auto
 
-definition "vle X Y \<equiv> \<exists>Z. X + Z = Y" 
+lemma zero_le [iff]: "0 \<le> X" by (subst le_iff_lt_or_eq) auto
 
+lemma lt_mem_leE:
+  assumes "X < Y"
+  obtains y where "y \<in> Y" "X \<le> y"
+  using assms unfolding le_iff_lt_or_eq lt_iff_mem_trans_closure by auto
 
+lemma lt_if_mem_if_le [trans]:
+  assumes "X \<le> Y"
+  and "Y \<in> Z"
+  shows "X < Z"
+  using assms mem_trans_closure_eq_bin_union_idx_union[of Z]
+  unfolding le_iff_lt_or_eq lt_iff_mem_trans_closure
+  by auto
+
+corollary lt_iff_bex_le: "X < Y \<longleftrightarrow> (\<exists>y \<in> Y. X \<le> y)"
+  by (auto elim: lt_mem_leE intro: lt_if_mem_if_le)
+
+lemma lt_if_lt_if_le [trans]:
+  assumes "X \<le> Y"
+  and "Y < Z"
+  shows "X < Z"
+  using assms mem_trans_closure_eq_bin_union_idx_union[of Z] mem_mem_trans_closure_trans
+  unfolding le_iff_lt_or_eq lt_iff_mem_trans_closure
+  by blast
+
+lemma lt_if_le_if_lt [trans]:
+  assumes "X < Y"
+  and "Y \<le> Z"
+  shows "X < Z"
+  using assms mem_trans_closure_eq_bin_union_idx_union[of Z] mem_mem_trans_closure_trans
+  unfolding le_iff_lt_or_eq lt_iff_mem_trans_closure
+  by blast
+
+lemma not_le_if_lt: "X < Y \<Longrightarrow> \<not>(Y \<le> X)"
+  using lt_trans le_iff_lt_or_eq by auto
+
+lemma not_lt_if_le: "X \<le> Y \<Longrightarrow> \<not>(Y < X)"
+  using not_le_if_lt by auto
+
+lemma antisymmetric_le: "antisymmetric (\<le>)"
+  unfolding le_iff_lt_or_eq using lt_trans by auto
+
+lemma ne_if_lt:
+  assumes "X < Y"
+  shows "X \<noteq> Y"
+  using assms by auto
+
+lemma lt_if_ne_if_le:
+  assumes "X \<le> Y"
+  and "X \<noteq> Y"
+  shows "X < Y"
+  using assms unfolding le_iff_lt_or_eq by auto
+
+corollary lt_iff_le_and_ne: "X < Y \<longleftrightarrow> X \<le> Y \<and> X \<noteq> Y"
+  using le_if_lt ne_if_lt lt_if_ne_if_le by blast
+
+lemma le_if_eq: "X = Y \<Longrightarrow> X \<le> Y"
+  by simp
+
+lemma not_lt_if_not_le_or_eq: "\<not>(X < Y) \<longleftrightarrow> \<not>(X \<le> Y) \<or> X = Y"
+  unfolding le_iff_lt_or_eq by auto
+
+local_setup \<open>
+  HOL_Order_Tac.declare_order {
+    ops = {eq = @{term \<open>(=) :: set \<Rightarrow> set \<Rightarrow> bool\<close>}, le = @{term \<open>(\<le>)\<close>}, lt = @{term \<open>(<)\<close>}},
+    thms = {trans = @{thm le_trans}, refl = @{thm le_self}, eqD1 = @{thm le_if_eq},
+      eqD2 = @{thm le_if_eq[OF sym]}, antisym = @{thm antisymmetricD[OF antisymmetric_le]},
+      contr = @{thm notE}},
+    conv_thms = {less_le = @{thm eq_reflection[OF lt_iff_le_and_ne]},
+      nless_le = @{thm eq_reflection[OF not_lt_if_not_le_or_eq]}}
+  }
+\<close>
 
 end
