HOTG/Arithmetics/Transfinite_Recursion.thy
@@ -1,0 +1,12 @@
+\<^marker>\<open>creator "Kevin Kappelmann"\<close>
+section \<open>Transfinite Recursion\<close>
+theory Transfinite_Recursion
+  imports
+    Functions_Restrict
+begin
+
+(*TODO: migrate definition from HOL*)
+axiomatization transrec :: "((set \<Rightarrow> 'a) \<Rightarrow> set \<Rightarrow> 'a) \<Rightarrow> set \<Rightarrow> 'a"
+  where transrec_eq: "transrec f X = f ((transrec f)\<restriction>\<^bsub>X\<^esub>) X"
+
+end
