HOTG/Comprehension.thy
@@ -8,6 +8,8 @@ theory Comprehension
     Order_Set
 begin
 
+unbundle no_HOL_ascii_syntax
+
 definition collect :: \<open>set \<Rightarrow> (set \<Rightarrow> bool) \<Rightarrow> set\<close>
   where "collect A P \<equiv> \<Union>{if P x then {x} else {} | x \<in> A}"
 
